start of proof of weber_contract

CaseStudies/Gathering/InR2/Weber/Weber_point.v
@@ -193,6 +193,17 @@ intros H. transitivity (list_sum (alls 0%R (length l))).
 + apply list_sum_le. induction l as [|x l IH] ; cbn ; auto.
   rewrite Forall_cons_iff in H. apply Forall2_cons ; intuition.
 Qed. 
+
+Lemma list_sum_map_opp {A : Type} (f : A -> R) l : 
+  (-(list_sum (map f l)) == list_sum (map (fun x => -(f x)) l))%R.
+Proof. Admitted.
+
+Lemma list_sum_map_add {A : Type} (f1 f2 : A -> R) l1 l2 : 
+  length l1 = length l2 -> 
+  (list_sum (map f1 l1) + list_sum (map f2 l2) == 
+    list_sum (map (fun '(x1, x2) => f1 x1 + f2 x2) (combine l1 l2)))%R.
+Proof. Admitted.
+
 (* This is the function that a weber point minimizes. *)
 Definition dist_sum points (x : R2) := 
   list_sum (List.map (dist x) points).
@@ -210,21 +221,18 @@ Qed.
 
 (* [argmin f P] is the set of elements that minimize [f] in the set [P],
  * when sets are represented by membership predicates. *)
-Definition argmin {A : Type} (f : A -> R) (P : A -> Prop) : A -> Prop := 
-  fun a => P a /\ forall b, P b -> (f a <= f b)%R.
+Definition argmin {A : Type} (f : A -> R) : A -> Prop := 
+  fun a => forall b, (f a <= f b)%R.
   
-Local Instance argmin_compat {A : Type} : Proper (equiv ==> equiv ==> @Logic.eq A ==> equiv) argmin.
+Local Instance argmin_compat {A : Type} : Proper (equiv ==> @eq A ==> iff) argmin.
 Proof using . 
-intros f g Hfg P P' HPP' a a' Haa'. unfold argmin.
-rewrite <-Haa'. setoid_rewrite <-HPP'. setoid_rewrite <-Hfg.
+intros f g Hfg a a' Haa'. unfold argmin.
+rewrite <-Haa'. setoid_rewrite <-Hfg.
 reflexivity.
 Qed.
 
-(* The trivial predicate true everywhere. *)
-Definition predT {A : Type} : A -> Prop := fun _ => True.
-
 (* The set of Weber points of a finite collection of points *)
-Definition Weber points : R2 -> Prop := argmin (dist_sum points) predT.
+Definition Weber points : R2 -> Prop := argmin (dist_sum points).
 
 (* [Weber] doesn't depend on the order of the points. *)
 Global Instance weber_compat : Proper (PermutationA equiv ==> equiv ==> iff) Weber.
@@ -263,8 +271,8 @@ Qed.
 Lemma weber_similarity_weak points w (f : similarity R2) : 
   Weber points w -> Weber (List.map f points) (f w).
 Proof.
-unfold Weber, argmin. intros [_ H]. split ; try now unfold predT.
-intros b _. rewrite <-(Bijection.section_retraction f b). 
+unfold Weber, argmin. intros H b. 
+rewrite <-(Bijection.section_retraction f b). 
 remember (Bijection.retraction f b) as b'.
 repeat rewrite dist_sum_similarity. apply Rmult_le_compat_l.
 + now apply Rlt_le, zoom_pos.
@@ -340,41 +348,167 @@ rewrite segment_sym. unfold segment. exists r. split.
   now rewrite minus_morph, mul_opp.
 Qed.
 
-(*Lemma half_line_mul_dir o d x t : 
-  (0 < t)%R -> (half_line o d x <-> half_line o (t * d)%VS x).
-Proof. 
-intros Ht. split ; intros [s [Hs Hx]] ; unfold half_line.
-+ exists (s / t)%R. split. 
-  - unfold Rdiv. now apply Rle_mult_inv_pos.
-  - rewrite Hx. f_equiv. rewrite mul_morph. f_equiv. unfold Rdiv.  
-    rewrite Rmult_assoc, Rinv_l ; lra.
-+ exists (s * t)%R. split.
-  - nra.
-  - rewrite Hx. f_equiv. now rewrite mul_morph.
-Qed.*)
-
 (* [contract ps ps' x] means that [ps'] is obtained from [ps] by moving
  * each point towards [x].*)
-Definition contract ps ps' x := 
+Definition contract ps ps' x : Prop := 
   Forall2 (fun p p' => segment x p p') ps ps'.
 
-Local Instance contract_compat : Proper (eqlistA equiv ==> eqlistA equiv ==> equiv ==> iff) contract.
-Proof. intros ? ? H1 ? ? H2 ? ? H3. unfold contract. Search Forall2 Proper. Admitted.
+Lemma segment_dist_weak x a b : 
+  segment a b x -> dist a b = (dist a x + dist x b)%R.
+Proof. 
+unfold segment. intros [t [Ht Hx]].
+assert (H1t : (0 <= 1 - t <= 1)%R). { lra. }
+pose (rt := exist (fun t => 0 <= t <= 1)%R t Ht).
+pose (r1t := exist (fun t => 0 <= t <= 1)%R (1 - t)%R H1t).
+assert (Hx1 : x == straight_path a b r1t).
+{ 
+cbn -[equiv mul RealVectorSpace.add opp]. unfold Rminus. 
+rewrite <-add_morph, mul_1, RealVectorSpace.add_assoc, add_sub.
+rewrite minus_morph, mul_distr_add, opp_distr_add, mul_opp, opp_opp.
+rewrite RealVectorSpace.add_assoc, RealVectorSpace.add_comm, Hx.
+f_equiv. unfold Rminus. rewrite <-add_morph, mul_1, minus_morph. reflexivity.
+}
+assert (Hx2 : x == straight_path b a rt).
+{
+cbn -[equiv mul RealVectorSpace.add opp]. rewrite Hx. 
+unfold Rminus. rewrite <-add_morph, mul_distr_add, mul_1, minus_morph, mul_opp.
+rewrite 2 RealVectorSpace.add_assoc. f_equiv. rewrite RealVectorSpace.add_comm.
+reflexivity.
+}
+rewrite Hx1 at 1. rewrite straight_path_dist_start.
+rewrite (dist_sym _ x), Hx2, straight_path_dist_start.
+cbn -[dist]. rewrite (dist_sym a b). lra.
+Qed.
 
-(* We can even move points onto the weber point, it will still be preserved. *)
-Lemma weber_contract ps ps' w : 
-  contract ps ps' w -> Weber ps w -> Weber ps' w.
-Proof. Admitted.
+Lemma segment_dist_sum a b x :
+  segment a b x <-> dist a b = (dist a x + dist x b)%R.
+Proof.
+split ; [apply segment_dist_weak|]. 
+case (a =?= b) as [Eab | NEab].
++ rewrite Eab, dist_same. rewrite dist_sym. intros Hdist. 
+  assert (H : dist x b = 0%R). { lra. }
+  rewrite dist_defined in H. rewrite H. apply segment_start.
++ intros Hdist. destruct (triang_ineq_eq _ _ _ Hdist) as [Hcol _].
+  apply colinear_exists_mul in Hcol. destruct Hcol as [t Hxa].
+  2: intros H ; apply NEab ; rewrite R2sub_origin in H ; now symmetry.
+  assert (Ht : (Rabs t + Rabs (t - 1) == 1)%R).
+  {
+    assert (Hxb : (x - b)%VS == ((t - 1) * (b - a))%VS).
+    { unfold Rminus. rewrite <-add_morph, minus_morph, mul_1, <-Hxa.
+      rewrite <-RealVectorSpace.add_assoc. f_equiv. 
+      now rewrite opp_distr_add, add_sub. }
+    rewrite (dist_sym x a), (dist_sym b a) in Hdist. repeat rewrite norm_dist in Hdist.
+    rewrite Hxa, Hxb in Hdist. repeat rewrite norm_mul in Hdist.
+    rewrite <-Rmult_plus_distr_r in Hdist.
+    rewrite <-(Rmult_1_l (norm (b - a)%VS)) in Hdist at 1. Search Rmult "reg".
+    apply Rmult_eq_reg_r in Hdist ; [now symmetry|].
+    rewrite norm_defined. intros H. apply NEab. rewrite R2sub_origin in H. now symmetry.
+  }
+  rewrite segment_sym. exists t. split.
+  - case (Rle_dec 0%R t) as [Rle_0t | NRle_0t] ; case (Rle_dec t 1%R) as [Rle_t1 | NRle_t1] ; [lra | exfalso ..]. 
+    * rewrite Rabs_pos_eq in Ht by auto. rewrite Rabs_pos_eq in Ht by lra.
+      assert (Ht1 : t == 1%R). { cbn in Ht |- *. lra. }
+      intuition.
+    * rewrite Rabs_left1 in Ht by lra. rewrite Rabs_left1 in Ht by lra.
+      assert (Ht0 : t == 0%R). { cbn in Ht |- *. lra. }
+      intuition.
+    * rewrite Rabs_left1 in Ht by lra. rewrite Rabs_pos_eq in Ht by lra. lra.
+  - unfold Rminus. rewrite <-add_morph, mul_1, minus_morph, <-mul_opp.
+    rewrite (RealVectorSpace.add_comm a), RealVectorSpace.add_assoc, <-mul_distr_add.
+    rewrite <-Hxa, <-RealVectorSpace.add_assoc, (RealVectorSpace.add_comm _ a), add_opp, add_origin_r.
+    reflexivity.
+Qed.
+
+Lemma segment_argmin x a b : segment x a b <-> argmin (fun y => (dist y b - dist y a)%R) x.
+Proof.
+split.
++ intros Hsegment y. rewrite segment_dist_sum in Hsegment. rewrite Hsegment.
+  unfold Rminus at 1. rewrite Ropp_plus_distr, <-Rplus_assoc, Rplus_opp_r, Rplus_0_l.
+  cut (dist y a <= dist y b + dist b a)%R. { lra. }
+  apply RealMetricSpace.triang_ineq.
++ unfold argmin. intros Hdist. rewrite segment_dist_sum.
+  apply Rle_antisym ; [apply RealMetricSpace.triang_ineq |]. 
+  specialize (Hdist b). rewrite dist_same, Rminus_0_l in Hdist.
+  lra.
+Qed.
+
+
+Lemma contract_argmin_weak ps ps' x : 
+  contract ps ps' x -> argmin (fun y => (dist_sum ps' y - dist_sum ps y)%R) x.
+Proof.
+intros Hcontract y. unfold dist_sum, Rminus.
+repeat rewrite list_sum_map_opp, list_sum_map_add.
+2, 3: now symmetry ; eapply Forall2_length, Hcontract.
+apply list_sum_le. rewrite Forall2_Forall, combine_map, Forall_map, Forall_forall by now rewrite 2 map_length.
+intros [a b] Hin. rewrite in_combine_id in Hin. destruct Hin as [<- Hin].
+destruct a as [p' p]. apply segment_argmin. assert (H := Hcontract). 
+revert H. unfold contract. rewrite Forall2_Forall, Forall_forall by eapply Forall2_length, Hcontract.
+intros H. specialize (H (p, p')). apply H. now rewrite in_combine_sym. 
+Qed.
+
+Lemma contract_argmin ps ps' x0 x : 
+  contract ps ps' x0 ->  
+  (contract ps ps' x <-> argmin (fun y => (dist_sum ps' y - dist_sum ps y)%R) x).
+Proof. 
+intros Hcontract0. split. 
++ apply contract_argmin_weak.
++ apply contract_argmin_weak in Hcontract0.
+  unfold dist_sum, Rminus, argmin in *.
+  rewrite list_sum_map_opp.
+2, 3: now symmetry ; eapply Forall2_length, Hcontract.
+Admitted.
+
+Lemma Rminus_eq0_iff x y : (x - y)%R = 0%R <-> x = y. 
+Proof. lra. Qed.
+
+Lemma Rle_minus_sim r1 r2 : (r1 <= r2)%R -> (0 <= r2 - r1)%R.
+Proof. lra. Qed.
+
+Lemma argmin_sum {A : Type} (f g : A -> R) x0 x :
+  argmin f x0 -> argmin g x0 -> 
+  (argmin (fun x => (f x + g x)%R)x <-> argmin f x /\ argmin g x).
+Proof. 
+intros Hf0 Hg0. split ; unfold argmin in *.
++ intros Hfg.
+  cut (f x = f x0 /\ g x = g x0). { intros [-> ->]. intuition. }
+  rewrite <-(Rminus_eq0_iff (f x)), <-(Rminus_eq0_iff (g x)).
+  apply Rplus_eq_R0.
+  - apply Rle_minus_sim, Hf0.
+  - apply Rle_minus_sim, Hg0.
+  - cut ((f x + g x)%R = (f x0 + g x0)%R). { lra. }
+    apply Rle_antisym ; [apply Hfg|].
+    apply Rplus_le_compat ; auto.    
++ intros [Hf Hg] y. apply Rplus_le_compat.
+  - apply Hf.
+  - apply Hg.
+Qed. 
 
 (* See the thesis of Zohir Bouzid, lemma 3.1.5. *)
 Lemma weber_contract_strong ps ps' w0 : 
   contract ps ps' w0 -> Weber ps w0 ->
   (forall w, Weber ps' w <-> (Weber ps w /\ contract ps ps' w)).
-Proof. Admitted. 
+Proof. 
+intros Hcontract0 Hweb0 w. rewrite contract_argmin in * ; eauto. unfold Weber in *.
+rewrite <-(argmin_sum _ Hweb0 Hcontract0). f_equiv. 
+intros x. rewrite Rplus_minus. reflexivity.
+Qed.
+
+(* We can even move points onto the weber point, it will still be preserved. *)
+Corollary weber_contract ps ps' w : 
+  contract ps ps' w -> Weber ps w -> Weber ps' w.
+Proof. 
+intros Hcontract Hweb. rewrite (weber_contract_strong Hcontract Hweb). intuition.
+Qed.
 
 (* See the thesis of Zohir Bouzid, corollary 3.1.1. *)
 Corollary weber_contract_unique ps ps' w : 
   contract ps ps' w -> OnlyWeber ps w -> OnlyWeber ps' w. 
-Proof. Admitted. 
+Proof.
+intros Hcontract [Hweb HwebU]. split.
++ rewrite (weber_contract_strong Hcontract Hweb). intuition.
++ intros w' Hweb'. apply HwebU. 
+  rewrite (weber_contract_strong Hcontract Hweb) in Hweb'.
+  intuition.
+Qed.
 
 End WeberPoint.
